coq/proof/SoundForgetMemoryCall.v
@@ -16,6 +16,7 @@ Import Opsem.
 
 Require Import TODO.
 Require Import Hints.
+Require Import Exprs.
 Require Import Postcond.
 Require Import Validator.
 Require Import GenericValues.
@@ -27,13 +28,175 @@ Require Import SoundBase.
 Set Implicit Arguments.
 
 
-Lemma forget_memory_call_Subset inv
-  : Hints.Invariant.Subset (ForgetMemoryCall.t inv) inv.
+Lemma forget_memory_call_unary_Subset inv
+  : Invariant.Subset_unary (ForgetMemoryCall.unary inv) inv.
 Proof.
+  unfold ForgetMemoryCall.unary. ss.
+  econs.
+  - ii. ss.
+    rewrite ExprPairSetFacts.filter_iff in *; try by solve_compat_bool.
+    des. eauto.
+  - split; ss.
+  - ii. ss.
+    rewrite AtomSetFacts.filter_iff in *; try by solve_compat_bool.
+    des. eauto.
+  - ii. ss.
+Qed.
+
+Lemma forget_memory_call_Subset inv
+  : Invariant.Subset (ForgetMemoryCall.t inv) inv.
+Proof.
+  unfold ForgetMemoryCall.t.
+  destruct inv.
+  econs; ss; apply forget_memory_call_unary_Subset.
+Qed.
+
+Lemma forget_memory_call_unique_implies_private inv x
+      (UNIQUE: AtomSetImpl.mem x (ForgetMemoryCall.unary inv).(Invariant.unique) = true)
+  : IdTSet.mem (Tag.physical, x) (ForgetMemoryCall.unary inv).(Invariant.private) = true.
+Proof.
+  unfold ForgetMemoryCall.unary in *. ss.
+  rewrite AtomSetFacts.filter_b in UNIQUE; try by solve_compat_bool.
+  des_bool. des. eauto.
+Qed.
+
+Lemma private_preserved_after_call
+      mem0 mem1 invmem0 invmem1
+      conf gmax public uniqs
+      (INCR : InvMem.Unary.le (InvMem.Unary.lift mem0 uniqs invmem0) invmem1)
+      (MEM : InvMem.Unary.sem conf gmax public mem1 invmem1)
+  : <<PRIVATE_PRESERVED: forall mc b o, In b invmem0.(InvMem.Unary.private) ->
+                                   mload_aux mem0 mc b o = mload_aux mem1 mc b o>>.
+Proof.
+  ii. inv INCR. ss.
+  inv MEM.
+  rewrite <- MEM_PARENT0; cycle 1.
+  { rewrite <- PRIVATE_PARENT.
+    apply in_app. eauto. }
+  apply MEM_PARENT. apply in_app. eauto.
+Qed.
+
+Lemma sem_expr_private_preserved
+      conf st0 invst0 invmem0 inv0 invmem1 mem1 uniqs
+      e e1 e2
+      (* gmax public *)
+      (STATE : InvState.Unary.sem conf st0 invst0 invmem0 inv0)
+      (* (MEM : InvMem.Unary.sem conf gmax public mem1 invmem1) *)
+      (IN_PRIVATE: ExprPairSet.In (e1, e2)
+                                  (ExprPairSet.filter
+                                     (ForgetMemoryCall.is_private_ExprPair inv0)
+                                     (Invariant.lessdef inv0)))
+      (PRIVATE_PRESERVED: forall (mc : list AST.memory_chunk) (b : mblock) (o : Z),
+          In b (InvMem.Unary.private invmem0) -> mload_aux (Mem st0) mc b o = mload_aux mem1 mc b o)
+      (EXP_EQ: e=e1 \/ e=e2)
+      (MEM_LE: InvMem.Unary.le (InvMem.Unary.lift st0.(Mem) uniqs invmem0) invmem1)
+  : InvState.Unary.sem_expr conf st0 invst0 e =
+    InvState.Unary.sem_expr conf (mkState st0.(EC) st0.(ECS) mem1) invst0 e.
+Proof.
+  destruct e; ss.
+  { (* gep *)
+    erewrite <- sem_list_valueT_eq_locals with (st0 := mkState st0.(EC) st0.(ECS) mem1); ss.
+  }
+  erewrite <- sem_valueT_eq_locals with (st0 := mkState st0.(EC) st0.(ECS) mem1); ss.
+  des_ifs.
+  unfold mload. des_ifs.
+  apply PRIVATE_PRESERVED.
+  apply ExprPairSetFacts.filter_iff in IN_PRIVATE; try by solve_compat_bool. desH IN_PRIVATE.
+  unfold ForgetMemoryCall.is_private_ExprPair in *.
+  des_bool. ss. unfold ForgetMemoryCall.is_private_Expr in *.
+  des.
+  - subst. destruct v; ss.
+    unfold ForgetMemoryCall.is_private_Expr.
+    inv STATE.
+    exploit PRIVATE; eauto.
+    { apply IdTSetFacts.mem_iff. eauto. }
+    i. des_ifs.
+  - subst. destruct v; ss.
+    unfold ForgetMemoryCall.is_private_Expr.
+    inv STATE.
+    exploit PRIVATE; eauto.
+    { apply IdTSetFacts.mem_iff. eauto. }
+    i. des_ifs.
+Qed.
+
+Lemma forget_memory_call_unary_sound
+      conf st0 mem1
+      gmax public0 public1
+      invmem0 invmem1
+      invst0 inv0
+      (MEM_LE : InvMem.Unary.le (InvMem.Unary.lift st0.(Mem)
+                                                   (memory_blocks_of conf st0.(EC).(Locals) inv0.(Invariant.unique))
+                                                   invmem0) invmem1)
+      (MEM_BEFORE_CALL: InvMem.Unary.sem conf gmax public0 st0.(Mem) invmem0)
+      (MEM_AFTER_CALL: InvMem.Unary.sem conf gmax public1 mem1 invmem1)
+      (STATE : InvState.Unary.sem conf st0 invst0 invmem0 inv0)
+  : <<STATE_UNARY: InvState.Unary.sem conf (mkState st0.(EC) st0.(ECS) mem1) invst0 invmem0 (ForgetMemoryCall.unary inv0)>> /\
+    <<MEM_UNARY: InvMem.Unary.sem conf gmax public1 mem1 invmem0>>.
+Proof.
+  hexploit private_preserved_after_call; eauto. intro PRIVATE_PRESERVED. des.
+  split.
+  { (* STATE *)
+    assert (STATE_CPY:=STATE).
+    inv STATE.
+    econs.
+    - (* lessdef *)
+      ii. destruct x as [e1 e2]. ss.
+      erewrite <- sem_expr_private_preserved in VAL1; eauto.
+      assert (X:= H).
+      apply ExprPairSetFacts.filter_iff in H; try by solve_compat_bool. des.
+      
+      exploit LESSDEF; eauto. i.
+      erewrite <- sem_expr_private_preserved; eauto.
+    - inv NOALIAS. rename NOALIAS0 into NOALIAS.
+      econs.
+      + (* DIFFBLOCK *)
+        i.
+        erewrite sem_valueT_eq_locals in VAL1.
+        { erewrite sem_valueT_eq_locals in VAL2.
+          { ss. exploit DIFFBLOCK; eauto. }
+          ss.
+        }
+        ss.
+      + (* NOALIAS *)
+        i.
+        erewrite sem_valueT_eq_locals in VAL1.
+        { erewrite sem_valueT_eq_locals in VAL2.
+          { ss. exploit NOALIAS; eauto. }
+          ss.
+        }
+        ss.
+    - ss. admit. (* call preserves private-unique? *)
+    - ss.
+    - ss.
+      inv MEM_LE.
+      admit. (* TODO: let invmem stores nextblock *)
+    - ss.
+  }
+  { (* MEM *)
+    inv MEM_BEFORE_CALL.
+    rename GLOBALS into GLOBALS_B.
+    rename WF into WF_B.
+    rename PRIVATE into PRIVATE_B.
+    rename PRIVATE_PARENT into PRIVATE_PARENT_B.
+    rename PRIVATE_DISJOINT into PRIVATE_DISJOINT_B.
+    rename MEM_PARENT into MEM_PARENT_B.
+    rename UNIQUE_PARENT into UNIQUE_PARENT_B.
+    rename UNIQUE_PARENT_GLOBALS into UNIQUE_PARENT_GLOBALS_B.
+    rename UNIQUE_PRIVATE_PARENT into UNIQUE_PRIVATE_PARENT_B.
+    inv MEM_AFTER_CALL.
+    econs; eauto.
+    - admit. (* nextblock - easy *)
+    - admit. (* nextblock - easy *)
+    - i. rewrite MEM_PARENT_B; eauto.
+      admit. (* let InvMem.Unary.le guarantee eq of mem_parent: easy *)
+      (* rewrite <- MEM_PARENT. *)
+      (* { assert (HH: st0.(Mem) = invmem1.(InvMem.Unary.mem_parent)). *)
+      (*   { inv MEM_LE. *)
+      (* { inv MEM_LE. ss. *)
+    - admit. (* unique_parent *)
+  }
 Admitted.
 
-(* Additionally, we should provide that all unique in (ForgetMemoryCall.t inv0) should be private *)
-(* TODO: ForgetMemoryCall should save private only, not unique *)
 Lemma forget_memory_call_sound
       conf_src st0_src id_src fun_src args_src cmds_src
       conf_tgt st0_tgt id_tgt fun_tgt args_tgt cmds_tgt
@@ -56,18 +219,40 @@ Lemma forget_memory_call_sound
          exists args1_tgt,
            <<ARGS_TGT: params2GVs conf_tgt.(CurTargetData) args_tgt st0_tgt.(EC).(Locals) conf_tgt.(Globals) = Some args1_tgt>> /\
            <<INJECT: list_forall2 (genericvalues_inject.gv_inject invmem0.(InvMem.Rel.inject)) args2_src args1_tgt>>)
-      (INCR: InvMem.Rel.le (InvMem.Rel.lift st0_src.(Mem) st0_tgt.(Mem) invmem0) invmem1)
+      (INCR: InvMem.Rel.le (InvMem.Rel.lift st0_src.(Mem) st0_tgt.(Mem)
+                                            (memory_blocks_of conf_src st0_src.(EC).(Locals) inv0.(Invariant.src).(Invariant.unique))
+                                            (memory_blocks_of conf_tgt st0_tgt.(EC).(Locals) inv0.(Invariant.tgt).(Invariant.unique))
+                                            invmem0) invmem1)
       (MEM_AFTER_CALL: InvMem.Rel.sem conf_src conf_tgt mem1_src mem1_tgt invmem1)
-  : exists invst2 invmem2,
+  : (* exists invst2  *) exists invmem2,
       <<INCR: InvMem.Rel.le invmem0 invmem2>> /\
       <<STATE:
         InvState.Rel.sem
           conf_src conf_tgt
           (mkState st0_src.(EC) st0_src.(ECS) mem1_src)
           (mkState st0_tgt.(EC) st0_tgt.(ECS) mem1_tgt)
-          invst2 invmem2 (ForgetMemoryCall.t inv0)>> /\
+          invst0 invmem2 (ForgetMemoryCall.t inv0)>> /\
       <<MEM: InvMem.Rel.sem conf_src conf_tgt mem1_src mem1_tgt invmem2>> /\
       <<MEM_INJ: invmem2.(InvMem.Rel.inject) = invmem1.(InvMem.Rel.inject)>>.
 Proof.
-  
-Admitted.
+  exists (InvMem.Rel.mk
+       invmem0.(InvMem.Rel.src) invmem0.(InvMem.Rel.tgt) invmem0.(InvMem.Rel.gmax) invmem1.(InvMem.Rel.inject)).
+
+  inv INCR. ss.
+  rename SRC into LE_SRC. rename TGT into LE_TGT.
+  inv STATE. inv MEM_BEFORE_CALL. inv MEM_AFTER_CALL.
+  rewrite GMAX in *.
+
+  exploit forget_memory_call_unary_sound; try exact LE_SRC; eauto. i. des.
+  exploit forget_memory_call_unary_sound; try exact LE_TGT; eauto. i. des.
+
+  esplits; eauto.
+  - econs; ss.
+  - econs; ss.
+    ii. exploit MAYDIFF; eauto. i.
+    erewrite sem_idT_eq_locals.
+    { des. esplits; eauto.
+      eapply genericvalues_inject.gv_inject_incr; eauto. }
+    ss.
+  - econs; ss.
+Qed.
